theories/automation.v
@@ -236,6 +236,7 @@ Ltac solve_normalize_bv_unsigned :=
   repeat match goal with | |- context [bv_wrap ?n ?x] => reduce_closed (bv_wrap n x) end;
   unfold block;
   bv_wrap_simplify_left;
+  lazymatch goal with | |- bv_wrap _ ?z = _ => ring_simplify z end;
   apply H.
 
 Global Hint Extern 10 (TacticHint (normalize_bv_unsigned _)) =>
@@ -730,19 +731,12 @@ Section instances.
   *)
   Lemma subsume_mem_uninit_mem_uninit a1 a2 n1 n2 G
         `{!BvSolve (0 ≤ n2 ∧ a1 ≤ a2 ∧ a2 + n2 ≤ a1 + n1)}:
-    (
-      (* tactic_hint (normalize_bv_unsigned (a2 - a1)) (λ m1, ⌜0 ≤ m1 < 2 ^ 64⌝ ∗ *)
-     (* tactic_hint (normalize_bv_unsigned (n1 - n2 - m1)) (λ m2, ⌜0 ≤ m2 < 2 ^ 64⌝ ∗ ( *)
-      a1 ↦ₘ? (a2 - a1) -∗
-     (a2 + n2) ↦ₘ? (n1 - n2 - (a2 - a1)) -∗ G) -∗
+    (tactic_hint (normalize_bv_unsigned (a2 - a1)) (λ m1, ⌜0 ≤ m1 < 2 ^ 64⌝ ∗
+     tactic_hint (normalize_bv_unsigned (n1 - n2 - m1)) (λ m2, ⌜0 ≤ m2 < 2 ^ 64⌝ ∗ (
+      a1 ↦ₘ? m1 -∗
+     (a2 + n2) ↦ₘ? m2 -∗ G)))) -∗
      subsume (a1 ↦ₘ? n1) (a2 ↦ₘ? n2) G.
-    (* (tactic_hint (normalize_bv_unsigned (a2 - a1)) (λ m1, ⌜0 ≤ m1 < 2 ^ 64⌝ ∗ *)
-    (*  tactic_hint (normalize_bv_unsigned (n1 - n2 - m1)) (λ m2, ⌜0 ≤ m2 < 2 ^ 64⌝ ∗ ( *)
-    (*   a1 ↦ₘ? m1 -∗ *)
-    (*  (a2 + n2) ↦ₘ? m2 -∗ G)))) -∗ *)
-    (*  subsume (a1 ↦ₘ? n1) (a2 ↦ₘ? n2) G. *)
-  Proof. Admitted.
-  (*
+  Proof.
     unfold BvSolve, normalize_bv_unsigned, tactic_hint in *. iIntros "HG Ha".
     iDestruct "HG" as "(%m1&%Hm1&%&%m2&%Hm2&%&HG)".
     have ? : 0 ≤ a1 ∧ a1 + n1 < 2 ^ 64 by admit.
@@ -752,7 +746,6 @@ Section instances.
     have -> : (n1 - m1 - n2) = m2 by bv_solve.
     iFrame. iApply ("HG" with "[$] [$]").
   Admitted.
-*)
   Global Instance subsume_mem_uninit_mem_uninit_inst a1 a2 n1 n2
          `{!BvSolve (0 ≤ n2 ∧ a1 ≤ a2 ∧ a2 + n2 ≤ a1 + n1)}:
     Subsume (a1 ↦ₘ? n1) (a2 ↦ₘ? n2) :=
@@ -764,21 +757,13 @@ Section instances.
   *)
   Lemma subsume_mem_uninit_mem_uninit2 a1 a2 n1 n2 G
         `{!BvSolve (0 ≤ n2 ∧ a1 ≤ a2 ∧ a2 ≤ a1 + n1 ∧ a1 + n1 ≤ a2 + n2)}:
-(
-    (* (tactic_hint (normalize_bv_unsigned (a2 - a1)) (λ m1, ⌜0 ≤ m1 < 2 ^ 64⌝ ∗ *)
-     (* tactic_hint (normalize_bv_unsigned (n2 - (n1 - (a2 - a1)))) (λ m2, ⌜0 ≤ m2 < 2 ^ 64⌝ ∗ *)
-     (* tactic_hint (normalize_bv_unsigned (a2 + n1 - (a2 - a1))) (λ m3, ⌜n2 < 2 ^ 64⌝ ∗ ( *)
-     a1 ↦ₘ? (a2 - a1) -∗
-     (a2 + n1 - (a2 - a1)) ↦ₘ? (n2 - (n1 - (a2 - a1))) ∗ G) -∗
+    (tactic_hint (normalize_bv_unsigned (a2 - a1)) (λ m1, ⌜0 ≤ m1 < 2 ^ 64⌝ ∗
+     tactic_hint (normalize_bv_unsigned (n2 - (n1 - m1))) (λ m2, ⌜0 ≤ m2 < 2 ^ 64⌝ ∗
+     tactic_hint (normalize_bv_unsigned (a2 + n1 - m1)) (λ m3, ⌜n2 < 2 ^ 64⌝ ∗ (
+     a1 ↦ₘ? m1 -∗
+     m3 ↦ₘ? m2 ∗ G))))) -∗
      subsume (a1 ↦ₘ? n1) (a2 ↦ₘ? n2) G.
-    (* (tactic_hint (normalize_bv_unsigned (a2 - a1)) (λ m1, ⌜0 ≤ m1 < 2 ^ 64⌝ ∗ *)
-    (*  tactic_hint (normalize_bv_unsigned (n2 - (n1 - m1))) (λ m2, ⌜0 ≤ m2 < 2 ^ 64⌝ ∗ *)
-    (*  tactic_hint (normalize_bv_unsigned (a2 + n1 - m1)) (λ m3, ⌜n2 < 2 ^ 64⌝ ∗ ( *)
-    (*  a1 ↦ₘ? m1 -∗ *)
-    (*  m3 ↦ₘ? m2 ∗ G))))) -∗ *)
-    (*  subsume (a1 ↦ₘ? n1) (a2 ↦ₘ? n2) G. *)
-  Proof. Admitted.
-  (*
+  Proof.
     unfold BvSolve, normalize_bv_unsigned, tactic_hint in *. iIntros "HG Ha".
     iDestruct "HG" as "(%m1&%Hm1&%&%m2&%Hm2&%&%m3&%Hm3&%&HG)".
     have ? : 0 ≤ a1 ∧ a1 + n1 < 2 ^ 64 by admit.
@@ -790,7 +775,6 @@ Section instances.
     have -> : (a2 + (n1 - m1)) = m3 by bv_solve.
     by have -> : (n2 - (n1 - m1)) = m2 by bv_solve.
   Admitted.
-*)
   Global Instance subsume_mem_uninit_mem_uninit2_inst a1 a2 n1 n2
         `{!BvSolve (0 ≤ n2 ∧ a1 ≤ a2 ∧ a2 ≤ a1 + n1 ∧ a1 + n1 ≤ a2 + n2)}:
     Subsume (a1 ↦ₘ? n1) (a2 ↦ₘ? n2) :=
